Download Link: https://assignmentchef.com/product/solved-dynamical-homework-9
<br>
<strong>1.1      Section 4.3 Problem 1.</strong>

Suppose <em>s</em><sub>1 </sub>and <em>s</em><sub>2 </sub>are simple function with <em>s</em><sub>1 </sub>= <em>s</em><sub>2 </sub>a.e. Let <em>E </em>be the set of measure 0 where <em>s</em><sub>1 </sub><em>6</em>= <em>s</em><sub>2</sub>. Observe that,

<em>n</em>

Z

<h2>s<sub>1</sub>dµ = <sup>X</sup>a<sub>i</sub>µ(A<sub>i</sub>)</h2>

<em>i</em>=1

<em>n</em>

<h2>= <sup>X</sup>a<sub>i</sub>µ(A<sub>i </sub> E) + aµ(E)</h2>

<em>i</em>=1

<em>n</em>

= <sup>X</sup><em>a<sub>i</sub>µ</em>(<em>A<sub>i </sub> E</em>) + <em>a · </em>0

<em>i</em>=1

<em>n</em>

<h2>= <sup>X</sup>a<sub>i</sub>µ(A<sub>i </sub> E)</h2>

<em>i</em>=1

and,

<em>m</em>

Z

<h2>s<sub>2</sub>dµ = <sup>X</sup>b<sub>i</sub>µ(B<sub>i</sub>)</h2>

<em>i</em>=1 <em>m</em>

<h2>= <sup>X</sup>b<sub>i</sub>µ(B<sub>i </sub> E) + bµ(E)</h2>

<em>i</em>=1 <em>m</em>

= <sup>X</sup><em>b<sub>i</sub>µ</em>(<em>B<sub>i </sub> E</em>) + <em>a · </em>0

<em>i</em>=1 <em>m</em>

<h2>= <sup>X</sup>b<sub>i</sub>µ(B<sub>i </sub> E)</h2>

<em>i</em>=1

But observe that <em>∪<sup>n</sup><sub>i</sub></em><sub>=1</sub><em>A<sub>i </sub>E </em><em>B<sub>i </sub>E </em>= <em>X E </em>and, by definition, <em>s</em><sub>1 </sub>= <em>s</em><sub>2 </sub>everywhere on this set. Since we are integrating the same function on the same set, we must have that <sup>R </sup><em>s</em><sub>1</sub><em>dµ </em>= <sup>R </sup><em>s</em><sub>2</sub><em>dµ</em>.

<strong>Problem 3.</strong>

Suppose <em>s </em>is a nonnegative simple function. Suppose <sup>R</sup><em><sub>X </sub>sdµ </em>= 0. Then,

<em>n</em>

Z

<h2>sdµ = <sup>X</sup>α<sub>i</sub>µ(E<sub>i</sub>)</h2>

<em><sup>x                 </sup></em><em>i</em>=1

= 0

Since <em>s ≥ </em>0, we have that <em>α<sub>i </sub>≥ </em>0 for all <em>i</em>. Moreover, we have that <em>µ</em>(<em>E<sub>i</sub></em>) <em>≥ </em>0 for all <em>i </em>by properties of measure. Thus, in order for this sum to equal 0, we must have that <em>α<sub>i</sub>µ</em>(<em>E<sub>i</sub></em>) = 0 for all <em>i</em>. Note that if <em>µ</em>(<em>E<sub>i</sub></em>) = 0 for all <em>i</em>, then <em>µ</em>(<em>X</em>) = 0. Hence, even if <em>s &gt; </em>0 on all of <em>X</em>, it is vacuously true that <em>s </em>= 0 a.e. since the whole space is measure 0. So let us assume that at least one <em>E<sub>i </sub></em>has positive measure. If <em>α<sub>i</sub>µ</em>(<em>E<sub>i</sub></em>) <em>&gt; </em>0 for this <em>i</em>, then <sup>P<em>n</em></sup><em><sub>i</sub></em><sub>=1 </sub><em>α<sub>i</sub>µ</em>(<em>E<sub>i</sub></em>) <em>&gt; </em>0, a contradiction. Hence, for every set <em>E<sub>i </sub></em>of positive measure, we must have that <em>s </em>= 0. Thus, <em>s </em>= 0 a.e. in <em>X</em>.

Now let us assume <em>s </em>= 0 a.e. in <em>X</em>. Then we have that there is a set <em>E </em>with <em>µ</em>(<em>E</em>) = 0 such that <em>s &gt; </em>0 on <em>E </em>and <em>s </em>= 0 on <em>X  E</em>. Since <em>s </em>= 0 a.e. and 0 is a simple function (with every coefficient <em>α<sub>i </sub></em>set to 0), we can apply Exercise 1 and state that we must have,

Z                    Z

<h2>                                                                                        sdµ =       0dµ</h2>

<em>X                    X n</em>

= <sup>X</sup>0 <em>· µ</em>(<em>A<sub>i</sub></em>)

<em>i</em>=1

= 0

as required.

<strong>1.2        Section 4.4</strong>

<strong>Problem 2.</strong>

Let <em>f </em>be a nonnegative measurable function and let <em>A </em>be a measurable set. Suppose <sup>R</sup><em>A f dµ </em>= 0. Then,

Z                                 Z

<em>f dµ </em>= sup<em>{            s dµ </em>: <em>s </em>is simple and 0 <em>≤ s ≤ f} </em>= 0

<em>A                                 A</em>

. Since the supremum of this set is 0 and every nonnegative simple function has a nonnegative integral, then for any <em>s </em>in the above set, we must have that,

<em>n</em>

Z

<h2>s dµ = <sup>X</sup>a<sub>i</sub>µ(A<sub>i</sub>)</h2>

<em><sup>A                    </sup></em><em>i</em>=1

= 0

By Section 4.3 Problem 3, we thus have that <em>s </em>= 0 a.e. in <em>A</em>. Since <em>s </em>was arbitrary, this holds for every <em>s </em>in the above set. Let us suppose that it is not the case that <em>f </em>= 0 a.e. That is, there is a set of positive measure where <em>f &gt; </em>0. Then there would be a simple function <em>s </em>with 0 <em>≤ s ≤ f </em>such that <em>s &gt; </em>0 on this set as well and hence it would not be the case that <em>s </em>= 0 a.e., a contradiction. Hence, we must have that <em>f </em>= 0 a.e.

Now suppose that <em>f </em>= 0 a.e. Then there is a set <em>E </em>of measure 0 such that <em>f </em>= 0 everywhere on <em>AE</em>. Fix a simple function <em>s </em>on <em>A </em>such that 0 <em>≤ s ≤ f</em>. For this to hold, we must have that <em>s </em>= 0 on <em>A  E</em>. We can have that 0 <em>&lt; s ≤ f </em>on <em>E</em>, but note that <em>µ</em>(<em>E</em>) = 0.

Thus,

<em>n</em>

Z

<h2>s = Xai µ(A<sub>i</sub>)</h2>

<em><sup>A            </sup></em><em>i</em>=1

<em>n                                       m</em>

<h2>= Xai µ(A<sub>i </sub> E) + <sup>X</sup>e<sub>i </sub>µ(E<sub>i</sub>)</h2>

<em>i</em>=1             <em>i</em>=1 <em>n</em>

<h2>= Xai µ(A<sub>i </sub> E)</h2>

<em>i</em>=1

= 0

where <em>∪E<sub>i </sub></em>= <em>E </em>(note since <em>E<sub>i </sub>⊂ E </em>we have <em>µ</em>(<em>E<sub>i</sub></em>) <em>≤ µ</em>(<em>E</em>) and since measure is nonneg-

ative and <em>µ </em>= 0, we get <em>µ</em>(<em>E<sub>i</sub></em>) = 0).

Since <em>s </em>was arbitrary on <em>A </em>with the property 0 <em>≤ s ≤ f</em>, this must hold for every element of the set <em>{</em><sup>R</sup><em><sub>A </sub>s dµ </em>: <em>s </em>is simple and 0 <em>≤ s ≤ f}</em>. Thus, <sup>R</sup><em><sub>A </sub>s </em>= 0 for every element <em>s </em>in the set and so,

Z                                 Z

<em>f dµ </em>= sup<em>{           s dµ </em>: <em>s </em>is simple and 0 <em>≤ s ≤ f}</em>

<em>A                                 A</em>

= 0

as required.

<strong>Problem 3.</strong>

Suppose <em>f </em>is a nonnegative measurable function and let <em>A,B </em>be measurable sets with <em>A ⊂ B</em>. We have that

Z                         Z

<em>f </em>= sup<em>{           s dµ </em>: <em>s </em>is simple and 0 <em>≤ s ≤ f}</em>

<em>A                         A</em>

and

Z                         Z

<em>f </em>= sup<em>{           s dµ </em>: <em>s </em>is simple and 0 <em>≤ s ≤ f}</em>

<em>B                         B</em>

Observe that for every <em>s </em>in the set <em>{</em><sup>R</sup><em><sub>B </sub>s dµ </em>: <em>s </em>is simple and 0 <em>≤ s ≤ f}</em>, we can write,

<em>n</em>

Z

<h2>s = <sup>X</sup>b<sub>n</sub>µ(B<sub>i</sub>)</h2>

<em><sup>B            </sup></em><em>i</em>=1

<em>n                                     m</em>

<h2>= <sup>X</sup>b<sub>i</sub>µ(B<sub>i </sub> A) + <sup>X</sup>a<sub>i</sub>µ(A<sub>i</sub>)</h2>

<em>i</em>=1                                  <em>i</em>=1

Z                  Z

<h2>                                                                            =           s +       s</h2>

<em>BA              A</em>

where <em>∪A<sub>i </sub></em>= <em>A</em>. Since the integral of any nonnegative simple function is nonnegative, we must have from the above that <sup>R</sup><em><sub>B </sub>s ≥ </em><sup>R</sup><em><sub>A </sub>s</em>. Observe that every element of <em>{</em><sup>R</sup><em><sub>A </sub>s dµ </em>: <em>s </em>is simple and 0 <em>≤ s ≤ f} </em>can be extended to a simple function on <em>B </em>by taking <em>s </em>= 0 on <em>B  A</em>, so we have <em>{</em><sup>R</sup><em><sub>A </sub>s dµ </em>: <em>s </em>is simple and 0 <em>≤ s ≤ f} ⊂ {</em><sup>R</sup><em><sub>B </sub>s dµ </em>: <em>s </em>is simple and 0 <em>≤ s ≤ f}</em>. Moreover, as we have shown above, if <sup>R</sup><em><sub>BA </sub>&gt; </em>0, then <sup>R</sup><em><sub>B </sub>s &gt; </em><sup>R</sup><em><sub>A </sub>s</em>. Thus, we must have that,

Z                                                                                                 Z

sup<em>{           s dµ </em>: <em>s </em>is simple and 0 <em>≤ s ≤ f} ≤ </em>sup<em>{               s dµ </em>: <em>s </em>is simple and 0 <em>≤ s ≤ f}</em>

<em>A         B </em>and so,

Z               Z

<h2>                                                                                                   f ≤        f</h2>

<em>A               B</em>

as required.

<strong>Problem 4.</strong>

Let <em>f </em>be a nonnegative measurable function and <em>{A<sub>j</sub>} </em>be a sequence of disjoint measurable sets. We have,

Z                                     Z

<em>f dµ </em>= sup<em>{              s dµ </em>: <em>s </em>is simple and 0 <em>≤ s ≤ f}</em>

<em>tA<sub>j                                                     </sub>tA<sub>j</sub></em>

Fix <em>s </em>in the above set. Then,

<em>n</em>

Z

<h2>s = <sup>X</sup>b<sub>i </sub>µ(B<sub>i</sub>) tAj i=1</h2>

for some sets <em>B<sub>i </sub></em>such that <em>∪B<sub>i </sub></em>= <em>tA<sub>j</sub></em>. However, we could alternatively divide up <em>tA<sub>j </sub></em>so that each subset in our sum corresponds to only one <em>A<sub>j</sub></em>. That is, we can write,

<em>n</em>

Z

<em>s </em>= XX<em>a</em><em>ji µ</em>(<em>A</em><em>ji</em>) <em><sup>tA</sup></em><em><sup>j                    </sup></em><em>j</em>=1 <em>i</em>=1

<em>n                                  n</em>

= X<em>a</em>1<em>i </em><em>µ</em>(<em>A</em>1<em>i</em>) + X<em>a</em>2<em>i </em><em>µ</em>(<em>A</em>2<em>i</em>) + <em>···</em>

<em>i</em>=1                               <em>i</em>=1

Z               Z

=         <em>s </em>+         <em>s </em>+ <em>···</em>

<em>A</em>1                     <em>A</em>2

Now note that <sup>R</sup><em><sub>A</sub></em><em><sub>i </sub>s </em>is contained in the above set for any <em>i </em>because we can set <sup>R</sup><em><sub>A</sub></em><em><sub>j </sub>s </em>= 0 for any <em>j 6</em>= <em>i </em>and maintain its status as a simple function. Hence,

<h3>                                                                             Z                                 Z</h3>

X

<em>f dµ </em>= <em>f dµ </em><em>tA</em><em>i                     </em><em>j A</em><em>j </em><strong>Problem 5.</strong>

Consider



<strong>1</strong>[0<em>,</em>1<em>/</em>2](<em>x</em>)      <em>n </em>odd

<em>f<sub>n</sub></em>(<em>x</em>) =

<strong>1</strong>[1<em>/</em>2<em>,</em>1](<em>x</em>)      <em>n </em>even

Observe that liminf<em><sub>n→∞ </sub>f<sub>n</sub></em>(<em>x</em>) = 0. Thus,

<h3>                                                                           Z                                           Z</h3>

liminf <em>f<sub>n</sub></em>(<em>x</em>)<em>dµ </em>=        0<em>dµ</em>

<em>n→∞</em>

= 0

Now note that <sup>R </sup><em>f<sub>n</sub>dµ </em>=  for all <em>n</em>. Thus,

Z

liminf      <em>f<sub>n</sub>dµ</em>

<em>n→∞                                n→∞ </em>2

Thus, we have that <sup>R </sup>liminf<em><sub>n→∞ </sub>f<sub>n</sub></em>(<em>x</em>)<em>dµ &lt; </em>liminf<em><sub>n→∞</sub></em><sup>R </sup><em>f<sub>n</sub>dµ </em>as required.